core/properties/monotonicity/Monotonicity.v
@@ -58,6 +58,7 @@ Proof.
     destruct H.
   - unfold TargetModel_elem_incl.
     simpl.
+    unfold instantiateTrOnModel ; simpl.
     crush.
     apply incl_l_nil in H.
     crush.
